backup for the change of fvar match

SEARind_tac.sml
@@ -1,0 +1,39 @@
+
+(*need to rely on the fact that the ind principle always have conclusion
+!a b. pred(a,b) ==> P(a,b)
+
+or !a:sort. P(a)
+
+where pred is not a fvar and P is 
+
+*)
+
+fun ind_with th (ct,asl,w) = 
+    let 
+        val (P,_) = dest_fvar $ concl (strip_all_and_imp th)
+        val (b,bvs) = strip_forall w
+        val th1 = fVar_Inst [(P,(bvs,b))] th
+    in match_mp_tac th1 (ct,asl,w)
+    end
+
+
+rewr_rule[Suc_def] N_ind_P
+
+EQ_psym "P" [assume “Eval(SUC,n) = Suc(n)”]
+rewr_fconv
+
+
+
+
+val l = 
+ fVar_Inst 
+[("P",([("b",mem_sort N)],
+ “Sub(Suc(a),Suc(b)) = Sub(a,b)”))] 
+ N_ind_P 
+
+val (ct, asl,w) = cg $ 
+e0
+(strip_tac >> ind_with N_ind_P >> )
+(form_goal
+ “!a b. Sub(Suc(a),Suc(b)) = Sub(a,b)”);
+
