SEARNarith.sml
@@ -1,4 +1,12 @@
 
+fun ind_with th (ct,asl,w) = 
+    let 
+        val (P,_) = dest_fvar $ concl (strip_all_and_imp th)
+        val (b,bvs) = strip_forall w
+        val th1 = fVar_Inst [(P,(bvs,b))] th
+    in match_mp_tac th1 (ct,asl,w)
+    end
+
 
 local
 val lemma = 
